@prefix : <https://cogito.iot.linkeddata.es/def/process#> .
@prefix owl: <http://www.w3.org/2002/07/owl#> .
@prefix rdf: <http://www.w3.org/1999/02/22-rdf-syntax-ns#> .
@prefix xml: <http://www.w3.org/XML/1998/namespace> .
@prefix xsd: <http://www.w3.org/2001/XMLSchema#> .
@prefix rdfs: <http://www.w3.org/2000/01/rdf-schema#> .
@prefix saref: <https://saref.etsi.org/core#> .
@prefix dcterms: <http://purl.org/dc/terms/> .
@prefix process: <https://cogito.iot.linkeddata.es/def/process#> .
@prefix facility: <https://cogito.iot.linkeddata.es/def/facility#> .
@prefix resource: <https://cogito.iot.linkeddata.es/def/resource#> .
@base <https://cogito.iot.linkeddata.es/def/process#> .

<https://cogito.iot.linkeddata.es/def/process#> rdf:type owl:Ontology ;
                                                 <http://purl.org/dc/elements/1.1/creator> "María Poveda Villalón" ,
                                                                                           "Raúl García Castro" ,
                                                                                           "Socorro  Bernardos Galindo" ;
                                                 <http://purl.org/dc/elements/1.1/description> "The COGITO Process ontology aims at modelling the construction process." ;
                                                 <http://purl.org/dc/elements/1.1/title> "Process Ontology" ;
                                                 dcterms:license <http://purl.org/NET/rdflicense/cc-by4.0> ;
                                                 owl:versionInfo "0.11.0" .

#################################################################
#    Annotation properties
#################################################################

###  http://purl.org/dc/elements/1.1/creator
<http://purl.org/dc/elements/1.1/creator> rdf:type owl:AnnotationProperty .


###  http://purl.org/dc/elements/1.1/description
<http://purl.org/dc/elements/1.1/description> rdf:type owl:AnnotationProperty .


###  http://purl.org/dc/elements/1.1/title
<http://purl.org/dc/elements/1.1/title> rdf:type owl:AnnotationProperty .


###  http://purl.org/dc/terms/license
dcterms:license rdf:type owl:AnnotationProperty .


#################################################################
#    Object Properties
#################################################################

###  https://cogito.iot.linkeddata.es/def/process#addsElement
process:addsElement rdf:type owl:ObjectProperty ;
                    owl:inverseOf process:isAddedByTask ;
                    rdfs:comment "A property that relates an entity (especially a process:Task) to the facility:Element it creates" ;
                    rdfs:label "adds element" .


###  https://cogito.iot.linkeddata.es/def/process#belongsToProcess
process:belongsToProcess rdf:type owl:ObjectProperty ;
                         owl:inverseOf process:hasTask ;
                         rdfs:range process:Process ;
                         rdfs:comment "A property that relates an entity (especially a process:Task) to the process:Process it belongs to" ;
                         rdfs:label "belongs to process" .


###  https://cogito.iot.linkeddata.es/def/process#controlsElement
process:controlsElement rdf:type owl:ObjectProperty ;
                        owl:inverseOf process:isControlledByTask ;
                        rdfs:range facility:Element ;
                        rdfs:comment "A property that relates an entity (especially a process:Task) to the facility:Element it controls" ;
                        rdfs:label "controls element" .


###  https://cogito.iot.linkeddata.es/def/process#hasComponentTask
process:hasComponentTask rdf:type owl:ObjectProperty ;
                         rdfs:range process:Task ;
                         rdfs:comment "A property that relates an entity (especially a process:WorkOrder) to its tasks" ;
                         rdfs:label "has component task" .


###  https://cogito.iot.linkeddata.es/def/process#hasCost
process:hasCost rdf:type owl:ObjectProperty ;
                rdfs:range process:Cost ;
                rdfs:comment "A property that relates an entity (especially a process:Task or a process:Process) to its cost" ;
                rdfs:label "has cost" .


###  https://cogito.iot.linkeddata.es/def/process#hasMainProvider
process:hasMainProvider rdf:type owl:ObjectProperty ;
                        rdfs:range resource:Worker ;
                        rdfs:comment "A property that relates an entity (especially a process:WorkOrder) to the resource:Worker that acts as its main provider" ;
                        rdfs:label "has main provider" .


###  https://cogito.iot.linkeddata.es/def/process#hasResourceTypeRequirement
process:hasResourceTypeRequirement rdf:type owl:ObjectProperty ;
                                   rdfs:range process:ResourceTypeRequirement ;
                                   rdfs:comment "Aproperty that relates an entity (especially a process:Task) to its requirements of resource types:" ;
                                   rdfs:label "has resource type requirement" .


###  https://cogito.iot.linkeddata.es/def/process#hasSubTask
process:hasSubTask rdf:type owl:ObjectProperty ;
                   owl:inverseOf process:isSubTaskOf ;
                   rdfs:range process:Task ;
                   rdfs:comment "A property that relates an entity (especially a process:Task) to the tasks it includes" ;
                   rdfs:label "has sub-task" .


###  https://cogito.iot.linkeddata.es/def/process#hasTask
process:hasTask rdf:type owl:ObjectProperty ;
                rdfs:range process:Task ;
                rdfs:comment "A property that relates an entity (especially a process:Process) to the tasks it involves" ;
                rdfs:label "has task" .


###  https://cogito.iot.linkeddata.es/def/process#hasWorkOrder
process:hasWorkOrder rdf:type owl:ObjectProperty ;
                     rdfs:range process:WorkOrder ;
                     rdfs:comment "A property that relates an entity (especially a process:Process) to the work orders it contains" ;
                     rdfs:label "has work order" .


###  https://cogito.iot.linkeddata.es/def/process#involvesResourceType
process:involvesResourceType rdf:type owl:ObjectProperty ;
                             rdfs:range resource:ResourceType ;
                             rdfs:comment "A property that relates an entity (especially a process:Process) to the resource types it includes" ;
                             rdfs:label "involves resource type" .


###  https://cogito.iot.linkeddata.es/def/process#isAddedByTask
process:isAddedByTask rdf:type owl:ObjectProperty ;
                      rdfs:range process:Task ;
                      rdfs:comment "A property that relates an entity (especially a  facility:Element) to the process:Task  that creates it" ;
                      rdfs:label "is added by task" .


###  https://cogito.iot.linkeddata.es/def/process#isControlledByTask
process:isControlledByTask rdf:type owl:ObjectProperty ;
                           rdfs:range process:Task ;
                           rdfs:comment "A property that relates an entity (especially a  facility:Element)  to the process:Task  that controls it" ;
                           rdfs:label "is controlled by task" .


###  https://cogito.iot.linkeddata.es/def/process#isExecutedAfter
process:isExecutedAfter rdf:type owl:ObjectProperty ;
                        rdfs:domain process:Task ;
                        rdfs:range process:Task ;
                        rdfs:comment "A property that relates an entity (especially a process:Task) to the task that have to be executed before it" ;
                        rdfs:label "is executed after" .


###  https://cogito.iot.linkeddata.es/def/process#isMeasuredIn
process:isMeasuredIn rdf:type owl:ObjectProperty ;
                     rdfs:range process:UnitOfCurrency ;
                     rdfs:comment "A property that relates an entity (especially a process:Cost) to the currency it is measured in" ;
                     rdfs:label "is measured in" .


###  https://cogito.iot.linkeddata.es/def/process#isRelatedToProcess
process:isRelatedToProcess rdf:type owl:ObjectProperty ;
                           owl:inverseOf process:isRelatedToProject ;
                           rdfs:range process:Process ;
                           rdfs:comment "A property that relates an entity (especially a facility:Project) to its processes" ;
                           rdfs:label "is related to process" .


###  https://cogito.iot.linkeddata.es/def/process#isRelatedToProject
process:isRelatedToProject rdf:type owl:ObjectProperty ;
                           rdfs:range facility:Project ;
                           rdfs:comment "A property that relates an entity (especially a process:Process) to its facility:Project" ;
                           rdfs:label "is related to project" .


###  https://cogito.iot.linkeddata.es/def/process#isRemovedByTask
process:isRemovedByTask rdf:type owl:ObjectProperty ;
                        owl:inverseOf process:removesElement ;
                        rdfs:range process:Task ;
                        rdfs:comment "A property that relates an entity (especially a  facility:Element)  to the process:Task  that removes it" ;
                        rdfs:label "is removed by task" .


###  https://cogito.iot.linkeddata.es/def/process#isRepairedByTask
process:isRepairedByTask rdf:type owl:ObjectProperty ;
                         owl:inverseOf process:repairsElelment ;
                         rdfs:range process:Task ;
                         rdfs:comment "A property that relates an entity (especially a  facility:Element)  to the process:Task  that repairs it" ;
                         rdfs:label "is repaired by task" .


###  https://cogito.iot.linkeddata.es/def/process#isSubTaskOf
process:isSubTaskOf rdf:type owl:ObjectProperty ;
                    rdfs:range process:Task ;
                    rdfs:comment "A property that relates an entity (especially a process:Task) to the task it belongs to" ;
                    rdfs:label "is sub-task of" .


###  https://cogito.iot.linkeddata.es/def/process#relatesToResourceType
process:relatesToResourceType rdf:type owl:ObjectProperty ;
                              rdfs:comment "A property that relates an entity (especially a process:ResourceTypeRequirement) to the resource type it refers to" ;
                              rdfs:label "relates to resource type" .


###  https://cogito.iot.linkeddata.es/def/process#removesElement
process:removesElement rdf:type owl:ObjectProperty ;
                       rdfs:range facility:Element ;
                       rdfs:comment "A property that relates a process:Task to the facility:Element it removes" ;
                       rdfs:label "removes element" .


###  https://cogito.iot.linkeddata.es/def/process#repairsElelment
process:repairsElelment rdf:type owl:ObjectProperty ;
                        rdfs:range facility:Element ;
                        rdfs:comment "A property that relates a process:Task to the facility:Element it repairs" ;
                        rdfs:label "repairs element" .


###  https://cogito.iot.linkeddata.es/def/resource#belongsToResourceType
resource:belongsToResourceType rdf:type owl:ObjectProperty ;
                               rdfs:range resource:ResourceType ;
                               rdfs:comment "A property that relates a resource:Resource to its type" ;
                               rdfs:label "belongs to resource type" .


###  https://cogito.iot.linkeddata.es/def/resource#hasAssignedResource
resource:hasAssignedResource rdf:type owl:ObjectProperty ;
                             rdfs:range resource:Resource ;
                             rdfs:comment "A property that relates an entity (especially a process:Task) to the resource:Resource it has assigned" ;
                             rdfs:label "has assigned resource" .


#################################################################
#    Data properties
#################################################################

###  http://purl.org/dc/terms/created
dcterms:created rdf:type owl:DatatypeProperty ;
                rdfs:isDefinedBy dcterms: ;
                rdfs:label <https://cogito.iot.linkeddata.es/def/created> .


###  http://purl.org/dc/terms/creator
dcterms:creator rdf:type owl:DatatypeProperty ;
                rdfs:isDefinedBy dcterms: ;
                rdfs:label "creator" .


###  http://purl.org/dc/terms/description
dcterms:description rdf:type owl:DatatypeProperty ;
                    rdfs:isDefinedBy "http://purl.org/dc/terms" ;
                    rdfs:label "description" .


###  http://purl.org/dc/terms/identifier
dcterms:identifier rdf:type owl:DatatypeProperty ;
                   rdfs:isDefinedBy dcterms: ;
                   rdfs:label "identifier" .


###  http://purl.org/dc/terms/title
dcterms:title rdf:type owl:DatatypeProperty ;
              rdfs:isDefinedBy dcterms: ;
              rdfs:label "title" .


###  https://cogito.iot.linkeddata.es/def/process#actualEndDate
process:actualEndDate rdf:type owl:DatatypeProperty ;
                      rdfs:comment "A property indicating the actual end date of an entity" ;
                      rdfs:label "actual end date" .


###  https://cogito.iot.linkeddata.es/def/process#actualStartDate
process:actualStartDate rdf:type owl:DatatypeProperty ;
                        rdfs:comment "A property indicating the actual start date of an entity" ;
                        rdfs:label "actual start date" .


###  https://cogito.iot.linkeddata.es/def/process#amount
process:amount rdf:type owl:DatatypeProperty ;
               rdfs:range xsd:float ;
               rdfs:comment "A property indicating the amount of an entity" ;
               rdfs:label "amount" .


###  https://cogito.iot.linkeddata.es/def/process#crewNumber
process:crewNumber rdf:type owl:DatatypeProperty ;
                   rdfs:comment "Property used as resource multiplier factor to specify the number of crews assigned to the task in order to do the work with the provided duration" ;
                   rdfs:label "crew number" .


###  https://cogito.iot.linkeddata.es/def/process#crewProductivity
process:crewProductivity rdf:type owl:DatatypeProperty ;
                         rdfs:comment "Property indicating  \"amount of work / unit of time\". At the moment, we only capture the list of elements to be built, so the productivity values we would use are \"units / time\". But, work quantity is typically measured as: m, m2, m3, units, depending on the type of activity. So, we could have a mixture of productivity metrics, m/time, m2/time, m3/time, depending on the type of activity." ;
                         rdfs:label "crew productivity" .


###  https://cogito.iot.linkeddata.es/def/process#crewProductivityPenalty
process:crewProductivityPenalty rdf:type owl:DatatypeProperty ;
                                rdfs:comment "Property used as factor to limit the maximum number of crew working in a task" ;
                                rdfs:label "crew productivity penalty" .


###  https://cogito.iot.linkeddata.es/def/process#currencyCode
process:currencyCode rdf:type owl:DatatypeProperty ;
                     rdfs:comment "A property indicating the currency code of an entity (especially a process:UnitOfCurrency)" ;
                     rdfs:label "currency code" .


###  https://cogito.iot.linkeddata.es/def/process#currencySymbol
process:currencySymbol rdf:type owl:DatatypeProperty ;
                       rdfs:comment "A property indicating the currency symbol of an entity (especially a process:UnitOfCurrency)" ;
                       rdfs:label "currency symbol" .


###  https://cogito.iot.linkeddata.es/def/process#duration
process:duration rdf:type owl:DatatypeProperty ;
                 rdfs:range xsd:nonNegativeInteger ;
                 rdfs:comment "A property indicating the minimal number of days doing a task takes" ;
                 rdfs:label "duration" .


###  https://cogito.iot.linkeddata.es/def/process#isCritical
process:isCritical rdf:type owl:DatatypeProperty ;
                   rdfs:range xsd:boolean ;
                   rdfs:comment "A property indicating if an entity (especially a task) is critical" ;
                   rdfs:label "is critical" .


###  https://cogito.iot.linkeddata.es/def/process#plannedEarlyEndDate
process:plannedEarlyEndDate rdf:type owl:DatatypeProperty ;
                            rdfs:range xsd:dateTimeStamp ;
                            rdfs:comment "A property indicating the earliest  date an entity can end" ;
                            rdfs:label "planned early end date" .


###  https://cogito.iot.linkeddata.es/def/process#plannedEarlyStartDate
process:plannedEarlyStartDate rdf:type owl:DatatypeProperty ;
                              rdfs:range xsd:dateTimeStamp ;
                              rdfs:comment "A property indicating the earliest  date an entity can start" ;
                              rdfs:label "planned early start date" .


###  https://cogito.iot.linkeddata.es/def/process#plannedEndDate
process:plannedEndDate rdf:type owl:DatatypeProperty ;
                       rdfs:range xsd:dateTime ;
                       rdfs:comment "A property indicating the planned end date of an entity" ;
                       rdfs:label "planned end date" .


###  https://cogito.iot.linkeddata.es/def/process#plannedLateEndDate
process:plannedLateEndDate rdf:type owl:DatatypeProperty ;
                           rdfs:range xsd:dateTimeStamp ;
                           rdfs:comment "A property indicating the latest  date an entity can end" ;
                           rdfs:label "planned late end date" .


###  https://cogito.iot.linkeddata.es/def/process#plannedLateStartDate
process:plannedLateStartDate rdf:type owl:DatatypeProperty ;
                             rdfs:range xsd:dateTimeStamp ;
                             rdfs:comment "A property indicating the latest  date an entity can start" ;
                             rdfs:label "planned late start date" .


###  https://cogito.iot.linkeddata.es/def/process#plannedStartDate
process:plannedStartDate rdf:type owl:DatatypeProperty ;
                         rdfs:range xsd:dateTime ;
                         rdfs:comment "A property indicating the planned start date of an entity" ;
                         rdfs:label "planned start date" .


###  https://cogito.iot.linkeddata.es/def/process#priority
process:priority rdf:type owl:DatatypeProperty ;
                 rdfs:range xsd:integer ;
                 rdfs:comment "A property indicating the priority of an entity" ;
                 rdfs:label "priority" .


###  https://cogito.iot.linkeddata.es/def/process#progress
process:progress rdf:type owl:DatatypeProperty ;
                 rdfs:range xsd:float ;
                 rdfs:comment "A property indicating the progress of an entity (especially a process:Task)" ;
                 rdfs:label "progress" .


###  https://cogito.iot.linkeddata.es/def/process#quantityNeeded
process:quantityNeeded rdf:type owl:DatatypeProperty ;
                       rdfs:comment "A property indicating the needed quantity of an entity" ;
                       rdfs:label "quantity needed" .


###  https://cogito.iot.linkeddata.es/def/process#result
process:result rdf:type owl:DatatypeProperty ;
               rdfs:comment "A property indicating the result of an entity (especially a process:Task)" ;
               rdfs:label "result" .


###  https://cogito.iot.linkeddata.es/def/process#status
process:status rdf:type owl:DatatypeProperty ;
               rdfs:comment "A property indicating the status of an entity (especially a process:WorkOrder and a process:Task)" ;
               rdfs:label "status" .


###  https://cogito.iot.linkeddata.es/def/process#timeStep
process:timeStep rdf:type owl:DatatypeProperty ;
                 rdfs:comment "A property indicating the time step of an entity (especially a process:Process)" ;
                 rdfs:label "time step" .


###  https://cogito.iot.linkeddata.es/def/process#timeWindow
process:timeWindow rdf:type owl:DatatypeProperty ;
                   rdfs:comment "A property indicating the time window of an entity (especially a process:Process)" ;
                   rdfs:label "time window" .


###  https://cogito.iot.linkeddata.es/def/process#totalFloat
process:totalFloat rdf:type owl:DatatypeProperty ;
                   rdfs:range xsd:nonNegativeInteger ;
                   rdfs:comment "A property indicating the number of days an entity (especially a task) can be delayed" ;
                   rdfs:label "total float" .


###  https://cogito.iot.linkeddata.es/def/process#validationMessage
process:validationMessage rdf:type owl:DatatypeProperty ;
                          rdfs:comment "A property indicating the validation message of an entity (especially a process:Task)" .


###  https://cogito.iot.linkeddata.es/def/process#workQuantity
process:workQuantity rdf:type owl:DatatypeProperty ;
                     rdfs:comment "Property  indicating  the amount of work. Work quantity is typically measured as: m, m2, m3, units, depending on the type of activity. So, we could have a mixture of productivity metrics, m/time, m2/time, m3/time, depending on the type of activity." ;
                     rdfs:label "work quantity" .


###  https://cogito.iot.linkeddata.es/def/process#workQuantityUnit
process:workQuantityUnit rdf:type owl:DatatypeProperty ;
                         rdfs:comment "Property indicating the unit used to measure wok quantity. Work quantity is typically measured as: m, m2, m3, units, depending on the type of activity." ;
                         rdfs:label "work quantity unit" .


#################################################################
#    Classes
#################################################################

###  https://cogito.iot.linkeddata.es/def/facility#Element
facility:Element rdf:type owl:Class ;
                 rdfs:comment "A subclass or bot:Element and, as such, a constituent of a construction entity with a characteristic technical function, form, or position" ;
                 rdfs:label "Element" .


###  https://cogito.iot.linkeddata.es/def/facility#Project
facility:Project rdf:type owl:Class ;
                 rdfs:comment "A large or major undertaking, especially one involving considerable money, personnel, and equipment" ;
                 rdfs:label "Project" .


###  https://cogito.iot.linkeddata.es/def/process#AsIsProcess
process:AsIsProcess rdf:type owl:Class ;
                    rdfs:subClassOf process:Process ;
                    rdfs:comment "A process in its current condition" ;
                    rdfs:label "As-is Process" .


###  https://cogito.iot.linkeddata.es/def/process#AsPlannedEnrichedProcess
process:AsPlannedEnrichedProcess rdf:type owl:Class ;
                                 rdfs:subClassOf process:Process ;
                                 rdfs:comment "A planned process after being enriched" ;
                                 rdfs:label "As-planned Enriched Process" .


###  https://cogito.iot.linkeddata.es/def/process#AsPlannedOriginalProcess
process:AsPlannedOriginalProcess rdf:type owl:Class ;
                                 rdfs:subClassOf process:Process ;
                                 rdfs:comment "An initial planned process" ;
                                 rdfs:label "As-planned Original Process" .


###  https://cogito.iot.linkeddata.es/def/process#ConstructionTask
process:ConstructionTask rdf:type owl:Class ;
                         rdfs:subClassOf process:Task ;
                         rdfs:comment "A task related to a construction domain" ;
                         rdfs:label "Construction Task" .


###  https://cogito.iot.linkeddata.es/def/process#Cost
process:Cost rdf:type owl:Class ;
             rdfs:comment "An entity representing the cost of another entity" ;
             rdfs:label "Cost" .


###  https://cogito.iot.linkeddata.es/def/process#GeometricQualityTask
process:GeometricQualityTask rdf:type owl:Class ;
                             rdfs:subClassOf process:Task ;
                             rdfs:comment "A task related to the geometric quaity domain" ;
                             rdfs:label "Geometric Quality Task" .


###  https://cogito.iot.linkeddata.es/def/process#Process
process:Process rdf:type owl:Class ;
                rdfs:comment "A series of actions aimed at accomplishing some result (in this case, related to a facility:Project)" ;
                rdfs:label "Process" .


###  https://cogito.iot.linkeddata.es/def/process#ResourceTypeRequirement
process:ResourceTypeRequirement rdf:type owl:Class ;
                                rdfs:comment "An entity that includes the requitrments that a task has pertaining a resource type" ;
                                rdfs:label "Resource Type Requirement" .


###  https://cogito.iot.linkeddata.es/def/process#SatetyAddingTask
process:SatetyAddingTask rdf:type owl:Class ;
                         rdfs:subClassOf process:Task ;
                         rdfs:comment "A task related to the safety domain that adds elements" ;
                         rdfs:label "Safety Adding Task" .


###  https://cogito.iot.linkeddata.es/def/process#SatetyRemovingTask
process:SatetyRemovingTask rdf:type owl:Class ;
                           rdfs:subClassOf process:Task ;
                           rdfs:comment "A task related to the safety domain that removes elements" ;
                           rdfs:label "Safety Removing Task" .


###  https://cogito.iot.linkeddata.es/def/process#Task
process:Task rdf:type owl:Class ;
             rdfs:comment "A piece of work, which is performed in a process:Process" ;
             rdfs:label "Task" .


###  https://cogito.iot.linkeddata.es/def/process#UnitOfCurrency
process:UnitOfCurrency rdf:type owl:Class ;
                       rdfs:comment "The currency used to measure a process:Cost" ;
                       rdfs:label "Unit of Currency" .


###  https://cogito.iot.linkeddata.es/def/process#VisualQualityTask
process:VisualQualityTask rdf:type owl:Class ;
                          rdfs:subClassOf process:Task ;
                          rdfs:comment "A task related to the visual quality domain" ;
                          rdfs:label "Visual Quality Task" .


###  https://cogito.iot.linkeddata.es/def/process#WorkOrder
process:WorkOrder rdf:type owl:Class ;
                  rdfs:comment "A command or instruction authorizing specific work, repairs, etc., to be done" ;
                  rdfs:label "Work Order" .


###  https://cogito.iot.linkeddata.es/def/resource#Resource
resource:Resource rdf:type owl:Class ;
                  rdfs:comment "A source of supply, support, or aid, especially one that can be readily drawn upon when needed" ;
                  rdfs:label "Resource" .


###  https://cogito.iot.linkeddata.es/def/resource#ResourceType
resource:ResourceType rdf:type owl:Class ;
                      rdfs:comment "The kind of resources assigned to a process:Task or involved in a process:Process" ;
                      rdfs:label "Resource Type" .


###  https://cogito.iot.linkeddata.es/def/resource#Worker
resource:Worker rdf:type owl:Class ;
                rdfs:subClassOf resource:Resource ;
                rdfs:comment "A human resource that works in a project (especially performing a process:Task)" ;
                rdfs:label "Worker" .


###  Generated by the OWL API (version 4.5.9.2019-02-01T07:24:44Z) https://github.com/owlcs/owlapi
